cleanq/crb: reworked proofs with new precond + starting of splitting write/reads even more
Signed-off-by: Roni Häcki <roni.haecki@inf.ethz.ch>

CleanQ/CleanQ_CRBModel_Complx.thy
@@ -28,6 +28,20 @@ subsection \<open>CleanQ Abstract Concurrent Ring Buffer Model State\<close>
 (* ==================================================================================== *)
 
 text \<open>
+  Previously we only defined that the ring contians "something".
+  Now we define the buffer itself as close as possible to the code 
+  we want to proof. 
+\<close>
+
+record CleanQ_Buffer =
+  region :: nat
+  offset :: nat
+  length :: nat
+  valid_offset :: nat
+  valid_length :: nat
+  flags :: nat
+
+text \<open>
   the model is exactly the same and we reuse the RB Model. 
 \<close>
 
@@ -35,11 +49,144 @@ text \<open>
 (* Define some global variables to make Simpl/Complex proofs work *)
 record CleanQ_CRB_State_vars = 
   CRB  :: "nat CleanQ_RB_State"
-  buf :: "nat"
+  buf_x :: "nat"
+  buf_y :: "nat"
   uni :: "nat set"
 (*>*)
 
+(* ------------------------------------------------------------------------------------ *)
+subsubsection \<open>Redifining writing/reading a buffer\<close>
+(* ------------------------------------------------------------------------------------ *)
 
+text \<open>
+   In reality the writes and reads to a buffer (or the buffer struct) are 
+   one per field and concurrent actions can happen during each write. In order
+   to model this, we redefine writing and reading a buffer to smaller steps 
+\<close>
+
+definition CleanQ_RB_read_tail_region_x :: "CleanQ_Buffer CleanQ_RB_State \<Rightarrow> nat" 
+  where "CleanQ_RB_read_tail_region_x rb = region (rb_read_tail (rTYX rb))"
+
+definition CleanQ_RB_read_tail_region_y :: "CleanQ_Buffer CleanQ_RB_State \<Rightarrow> nat" 
+  where "CleanQ_RB_read_tail_region_y rb = region (rb_read_tail (rTXY rb))"
+
+definition CleanQ_RB_read_tail_offset_x :: "CleanQ_Buffer CleanQ_RB_State \<Rightarrow> nat" 
+  where "CleanQ_RB_read_tail_offset_x rb = offset (rb_read_tail (rTYX rb))"
+
+definition CleanQ_RB_read_tail_offset_y :: "CleanQ_Buffer CleanQ_RB_State \<Rightarrow> nat" 
+  where "CleanQ_RB_read_tail_offset_y rb = offset (rb_read_tail (rTXY rb))"
+
+definition CleanQ_RB_read_tail_length_x :: "CleanQ_Buffer CleanQ_RB_State \<Rightarrow> nat" 
+  where "CleanQ_RB_read_tail_length_x rb = length (rb_read_tail (rTYX rb))"
+
+definition CleanQ_RB_read_tail_length_y :: "CleanQ_Buffer CleanQ_RB_State \<Rightarrow> nat" 
+  where "CleanQ_RB_read_tail_length_y rb = length (rb_read_tail (rTXY rb))"
+
+definition CleanQ_RB_read_tail_valid_offset_x :: "CleanQ_Buffer CleanQ_RB_State \<Rightarrow> nat" 
+  where "CleanQ_RB_read_tail_valid_offset_x rb = valid_offset (rb_read_tail (rTYX rb))"
+
+definition CleanQ_RB_read_tail_valid_offset_y :: "CleanQ_Buffer CleanQ_RB_State \<Rightarrow> nat" 
+  where "CleanQ_RB_read_tail_valid_offset_y rb = valid_offset (rb_read_tail (rTXY rb))"
+
+definition CleanQ_RB_read_tail_valid_length_x :: "CleanQ_Buffer CleanQ_RB_State \<Rightarrow> nat" 
+  where "CleanQ_RB_read_tail_valid_length_x rb = valid_length (rb_read_tail (rTYX rb))"
+
+definition CleanQ_RB_read_tail_valid_length_y :: "CleanQ_Buffer CleanQ_RB_State \<Rightarrow> nat" 
+  where "CleanQ_RB_read_tail_valid_length_y rb = valid_length (rb_read_tail (rTXY rb))"
+
+definition CleanQ_RB_read_tail_flags_x :: "CleanQ_Buffer CleanQ_RB_State \<Rightarrow> nat" 
+  where "CleanQ_RB_read_tail_flags_x rb = flags (rb_read_tail (rTYX rb))"
+
+definition CleanQ_RB_read_tail_flags_y :: "(CleanQ_Buffer CleanQ_RB_State) \<Rightarrow> nat" 
+  where "CleanQ_RB_read_tail_flags_y rb = flags (rb_read_tail (rTXY rb))"
+
+text \<open>
+  Show equality 
+\<close>
+
+lemma CleanQ_RB_read_tail_x_fields_eq :
+  shows "CleanQ_RB_read_tail_x rb =  buffer \<lparr> region := CleanQ_RB_read_tail_region_x rb, 
+                       offset := CleanQ_RB_read_tail_offset_x rb,
+                       length := CleanQ_RB_read_tail_length_x rb,
+                       valid_offset := CleanQ_RB_read_tail_valid_offset_x rb,
+                       valid_length := CleanQ_RB_read_tail_valid_length_x rb,
+                       flags := CleanQ_RB_read_tail_flags_x rb\<rparr>"
+  unfolding CleanQ_RB_read_tail_x_def CleanQ_RB_read_tail_region_x_def 
+    CleanQ_RB_read_tail_offset_x_def CleanQ_RB_read_tail_length_x_def 
+    CleanQ_RB_read_tail_valid_length_x_def CleanQ_RB_read_tail_valid_offset_x_def
+    CleanQ_RB_read_tail_flags_x_def 
+  by simp 
+
+lemma CleanQ_RB_read_tail_y_fields_eq :
+  shows "CleanQ_RB_read_tail_y rb =  buffer \<lparr> region := CleanQ_RB_read_tail_region_y rb, 
+                       offset := CleanQ_RB_read_tail_offset_y rb,
+                       length := CleanQ_RB_read_tail_length_y rb,
+                       valid_offset := CleanQ_RB_read_tail_valid_offset_y rb,
+                       valid_length := CleanQ_RB_read_tail_valid_length_y rb,
+                       flags := CleanQ_RB_read_tail_flags_y rb\<rparr>"
+  unfolding CleanQ_RB_read_tail_y_def CleanQ_RB_read_tail_region_y_def 
+    CleanQ_RB_read_tail_offset_y_def CleanQ_RB_read_tail_length_y_def 
+    CleanQ_RB_read_tail_valid_length_y_def CleanQ_RB_read_tail_valid_offset_y_def
+    CleanQ_RB_read_tail_flags_y_def 
+  by simp 
+
+(* ------------------------------------------------------------------------------------ *)
+subsubsection \<open>Defining enqueue and deuque for Complx\<close>
+(* ------------------------------------------------------------------------------------ *)
+
+
+abbreviation "CleanQ_CRB_enq_x b \<equiv> 
+            \<lbrace> CleanQ_RB_Invariants \<acute>uni \<acute>CRB  \<rbrace>
+            IF CleanQ_RB_enq_x_possible \<acute>CRB \<and> b \<in> rSX \<acute>CRB
+            THEN
+              \<lbrace> CleanQ_RB_enq_x_P \<acute>uni \<acute>CRB b \<rbrace>
+                \<acute>CRB := (CleanQ_RB_write_head_x b \<acute>CRB) ;;
+              \<lbrace> CleanQ_RB_enq_x_Q \<acute>uni \<acute>CRB b \<rbrace>
+                \<acute>CRB := (CleanQ_RB_incr_head_x b \<acute>CRB)
+            ELSE 
+                \<lbrace>  CleanQ_RB_Invariants \<acute>uni \<acute>CRB \<rbrace>
+                SKIP
+            FI"
+
+abbreviation "CleanQ_CRB_enq_y b \<equiv> 
+            \<lbrace> CleanQ_RB_Invariants \<acute>uni \<acute>CRB  \<rbrace>
+            IF CleanQ_RB_enq_y_possible \<acute>CRB \<and> b \<in> rSY \<acute>CRB
+            THEN
+              \<lbrace> CleanQ_RB_enq_y_P \<acute>uni \<acute>CRB b \<rbrace>
+                \<acute>CRB := (CleanQ_RB_write_head_y b \<acute>CRB) ;;
+              \<lbrace> CleanQ_RB_enq_y_Q \<acute>uni \<acute>CRB b \<rbrace>
+                \<acute>CRB := (CleanQ_RB_incr_head_y b \<acute>CRB)
+            ELSE 
+                \<lbrace>  CleanQ_RB_Invariants \<acute>uni \<acute>CRB \<rbrace>
+                SKIP
+            FI"
+
+abbreviation "CleanQ_CRB_deq_x \<equiv> 
+            \<lbrace> CleanQ_RB_Invariants \<acute>uni \<acute>CRB  \<rbrace>
+            IF CleanQ_RB_deq_x_possible \<acute>CRB
+            THEN
+              \<lbrace> CleanQ_RB_deq_x_P \<acute>uni \<acute>CRB (CleanQ_RB_read_tail_x \<acute>CRB) \<rbrace>
+                \<acute>buf_x := (CleanQ_RB_read_tail_x  \<acute>CRB) ;;
+              \<lbrace> CleanQ_RB_deq_x_Q \<acute>uni \<acute>CRB \<acute>buf_x \<rbrace>
+                \<acute>CRB := (CleanQ_RB_incr_tail_x \<acute>buf_x \<acute>CRB)
+            ELSE 
+                \<lbrace>  CleanQ_RB_Invariants \<acute>uni \<acute>CRB \<rbrace>
+                SKIP
+            FI"
+
+
+abbreviation "CleanQ_CRB_deq_y \<equiv> 
+            \<lbrace> CleanQ_RB_Invariants \<acute>uni \<acute>CRB  \<rbrace>
+            IF CleanQ_RB_deq_y_possible \<acute>CRB
+            THEN
+              \<lbrace> CleanQ_RB_deq_y_P \<acute>uni \<acute>CRB (CleanQ_RB_read_tail_y \<acute>CRB) \<rbrace>
+                \<acute>buf_y := (CleanQ_RB_read_tail_y  \<acute>CRB) ;;
+              \<lbrace> CleanQ_RB_deq_y_Q \<acute>uni \<acute>CRB \<acute>buf_y \<rbrace>
+                \<acute>CRB := (CleanQ_RB_incr_tail_y \<acute>buf_y \<acute>CRB)
+            ELSE 
+                \<lbrace>  CleanQ_RB_Invariants \<acute>uni \<acute>CRB \<rbrace>
+                SKIP
+            FI"
 
 (* ------------------------------------------------------------------------------------ *)
 subsubsection \<open>Hoare Triples for the Enqueue Operation\<close>
@@ -148,17 +295,17 @@ text \<open>
 
 lemma  CleanQ_RB_read_tail_x_hoare:
  "\<Gamma>, \<Theta> |\<turnstile>\<^bsub>/ F\<^esub>  
-  \<lbrace> CleanQ_RB_deq_x_P K \<acute>CRB \<acute>buf \<rbrace> 
-    \<acute>buf := (CleanQ_RB_read_tail_x \<acute>CRB)
-  \<lbrace> CleanQ_RB_deq_x_Q K \<acute>CRB \<acute>buf  \<rbrace>, \<lbrace>True\<rbrace>"  
+  \<lbrace> CleanQ_RB_deq_x_P K \<acute>CRB \<acute>buf_x \<rbrace> 
+    \<acute>buf_x := (CleanQ_RB_read_tail_x \<acute>CRB)
+  \<lbrace> CleanQ_RB_deq_x_Q K \<acute>CRB \<acute>buf_x  \<rbrace>, \<lbrace>True\<rbrace>"  
   by(oghoare, auto)
   
 
 lemma  CleanQ_RB_read_tail_y_hoare:
   "\<Gamma>, \<Theta> |\<turnstile>\<^bsub>/ F\<^esub>  
-  \<lbrace> CleanQ_RB_deq_y_P K \<acute>CRB \<acute>buf \<rbrace> 
-    \<acute>buf := (CleanQ_RB_read_tail_y \<acute>CRB)
-  \<lbrace> CleanQ_RB_deq_y_Q K \<acute>CRB \<acute>buf  \<rbrace>, \<lbrace>True\<rbrace>"  
+  \<lbrace> CleanQ_RB_deq_y_P K \<acute>CRB \<acute>buf_y \<rbrace> 
+    \<acute>buf_y := (CleanQ_RB_read_tail_y \<acute>CRB)
+  \<lbrace> CleanQ_RB_deq_y_Q K \<acute>CRB \<acute>buf_y  \<rbrace>, \<lbrace>True\<rbrace>"  
   by(oghoare, auto)  
 
 paragraph \<open>Incrementing the Tail Pointer\<close>
@@ -172,9 +319,10 @@ lemma  CleanQ_RB_incr_tail_x_hoare:
     \<lbrace>  CleanQ_RB_deq_x_Q K \<acute>CRB b \<rbrace> 
         \<acute>CRB := (CleanQ_RB_incr_tail_x b \<acute>CRB)
     \<lbrace> CleanQ_RB_deq_x_R K \<acute>CRB b\<rbrace>,\<lbrace>True\<rbrace>" 
-  apply(oghoare)
-  using CleanQ_RB_deq_x_all_inv by fastforce
-
+  apply(oghoare, auto)
+  using CleanQ_RB_deq_x_all_inv by blast
+  
+  
 
 lemma  CleanQ_RB_incr_tail_y_hoare:
    "\<Gamma>, \<Theta> |\<turnstile>\<^bsub>/ F\<^esub> 
@@ -193,38 +341,37 @@ text \<open>
 
 lemma CleanQ_RB_deq_x_hoare : 
    "\<Gamma>, \<Theta> |\<turnstile>\<^bsub>/ F\<^esub>  
-    \<lbrace>  CleanQ_RB_deq_x_P K \<acute>CRB bf \<rbrace> 
-      \<acute>buf := (CleanQ_RB_read_tail_x \<acute>CRB) ;;
-    \<lbrace> CleanQ_RB_deq_x_Q K \<acute>CRB bf  \<rbrace>
-      \<acute>CRB := (CleanQ_RB_incr_tail_x bf \<acute>CRB)
-    \<lbrace> CleanQ_RB_deq_x_R K \<acute>CRB bf \<rbrace>, \<lbrace>True\<rbrace>"
+    \<lbrace>  CleanQ_RB_deq_x_P K \<acute>CRB (CleanQ_RB_read_tail_x \<acute>CRB) \<rbrace> 
+      \<acute>buf_x := (CleanQ_RB_read_tail_x \<acute>CRB) ;;
+    \<lbrace> CleanQ_RB_deq_x_Q K \<acute>CRB \<acute>buf_x  \<rbrace>
+      \<acute>CRB := (CleanQ_RB_incr_tail_x \<acute>buf_x \<acute>CRB)
+    \<lbrace> CleanQ_RB_deq_x_R K \<acute>CRB \<acute>buf_x \<rbrace> , \<lbrace>True\<rbrace>"
   apply(oghoare, auto)
   using CleanQ_RB_deq_x_all_inv by blast
   
-
+  
 lemma CleanQ_RB_deq_y_hoare : 
    "\<Gamma>, \<Theta> |\<turnstile>\<^bsub>/ F\<^esub>   
-    \<lbrace>  CleanQ_RB_deq_y_P K \<acute>CRB bf \<rbrace> 
-      \<acute>buf := (CleanQ_RB_read_tail_y \<acute>CRB) ;;
-    \<lbrace> CleanQ_RB_deq_y_Q K \<acute>CRB bf  \<rbrace>
-      \<acute>CRB := (CleanQ_RB_incr_tail_y bf \<acute>CRB)
-    \<lbrace> CleanQ_RB_deq_y_R K \<acute>CRB bf \<rbrace>, \<lbrace>True\<rbrace>"
+    \<lbrace>  CleanQ_RB_deq_y_P K \<acute>CRB (CleanQ_RB_read_tail_x \<acute>CRB) \<rbrace> 
+      \<acute>buf_y := (CleanQ_RB_read_tail_y \<acute>CRB) ;;
+    \<lbrace> CleanQ_RB_deq_y_Q K \<acute>CRB \<acute>buf_y  \<rbrace>
+      \<acute>CRB := (CleanQ_RB_incr_tail_y \<acute>buf_y \<acute>CRB)
+    \<lbrace> CleanQ_RB_deq_y_R K \<acute>CRB \<acute>buf_y \<rbrace>, \<lbrace>True\<rbrace>"
   apply(oghoare, auto)
   using CleanQ_RB_deq_y_all_inv by blast
   
-
-
+  
 type_synonym funcs = "string \<times> nat"
 
 lemma CleanQ_RB_read_concurent:
      "\<Gamma>, \<Theta> |\<turnstile>\<^bsub>/F\<^esub>   
       COBEGIN
          \<lbrace>  CleanQ_RB_Invariants \<acute>uni \<acute>CRB \<rbrace>
-           \<acute>buf := CleanQ_RB_read_head_x \<acute>CRB
+           \<acute>buf_x := CleanQ_RB_read_head_x \<acute>CRB
          \<lbrace>  CleanQ_RB_Invariants \<acute>uni \<acute>CRB \<rbrace>, \<lbrace>True\<rbrace>
          \<parallel> 
          \<lbrace>  CleanQ_RB_Invariants \<acute>uni \<acute>CRB \<rbrace>
-          \<acute>buf := CleanQ_RB_read_head_y \<acute>CRB
+          \<acute>buf_y := CleanQ_RB_read_head_y \<acute>CRB
          \<lbrace>  CleanQ_RB_Invariants \<acute>uni \<acute>CRB \<rbrace>, \<lbrace>True\<rbrace>
       COEND
       \<lbrace>  CleanQ_RB_Invariants \<acute>uni \<acute>CRB \<rbrace>, \<lbrace>True\<rbrace>"
@@ -233,91 +380,6 @@ lemma CleanQ_RB_read_concurent:
 
 (* let's try this... I think we could start with this and showing this for all
   four combinations. Then continue with splitting up *)
-
-
-lemma CleanQ_RB_enq_enq:
-     "\<Gamma>, \<Theta> |\<turnstile>\<^bsub>/F\<^esub>   
-      COBEGIN
-         \<lbrace>  CleanQ_RB_enq_x_P \<acute>uni \<acute>CRB bx \<rbrace>
-           \<acute>CRB := CleanQ_RB_enq_x bx \<acute>CRB
-         \<lbrace>  CleanQ_RB_enq_x_R \<acute>uni \<acute>CRB bx \<rbrace>, \<lbrace>True\<rbrace>
-         \<parallel> 
-         \<lbrace>  CleanQ_RB_enq_y_P \<acute>uni \<acute>CRB by \<rbrace>
-          \<acute>CRB := CleanQ_RB_enq_y by \<acute>CRB 
-         \<lbrace>  CleanQ_RB_enq_y_R \<acute>uni \<acute>CRB by \<rbrace>, \<lbrace>True\<rbrace>
-      COEND
-      \<lbrace>  CleanQ_RB_Invariants \<acute>uni \<acute>CRB \<rbrace>, \<lbrace>True\<rbrace>"
-  apply(oghoare, auto)
-  apply(simp_all add :CleanQ_RB_enq_x_inv_all) 
-  apply(simp_all add :CleanQ_RB_enq_y_inv_all) 
-  apply (simp add: CleanQ_RB_enq_x_def CleanQ_RB_enq_y_possible_def)
-  apply (simp add: CleanQ_RB_enq_y_enq_x_possible)
-  apply (simp add: CleanQ_RB_enq_y_result)
-  by (simp add: CleanQ_RB_enq_x_result)
-
-lemma CleanQ_RB_enq_deq:
-     "\<Gamma>, \<Theta> |\<turnstile>\<^bsub>/F\<^esub>   
-      COBEGIN
-         \<lbrace>  CleanQ_RB_enq_x_P \<acute>uni \<acute>CRB bx \<rbrace>
-           \<acute>CRB := CleanQ_RB_enq_x bx \<acute>CRB
-         \<lbrace>  CleanQ_RB_enq_x_R \<acute>uni \<acute>CRB bx \<rbrace>, \<lbrace>True\<rbrace>
-         \<parallel> 
-         \<lbrace>  CleanQ_RB_deq_y_P \<acute>uni \<acute>CRB by \<rbrace>
-          \<acute>CRB := CleanQ_RB_deq_y \<acute>CRB 
-         \<lbrace>  CleanQ_RB_deq_y_R \<acute>uni \<acute>CRB by \<rbrace>, \<lbrace>True\<rbrace>
-      COEND
-      \<lbrace>  CleanQ_RB_Invariants \<acute>uni \<acute>CRB \<rbrace>, \<lbrace>True\<rbrace>"
-  apply(oghoare, auto)
-  apply(simp_all add :CleanQ_RB_enq_x_inv_all) 
-  apply(simp_all add :CleanQ_RB_deq_y_all_inv)
-  apply (simp add: CleanQ_RB_enq_x_deq_y_possible)
-  apply (simp add: CleanQ_RB_deq_y_enq_x_possible)
-  by (simp add: CleanQ_RB_enq_x_result)
-  
-lemma CleanQ_RB_deq_enq:
-     "\<Gamma>, \<Theta> |\<turnstile>\<^bsub>/F\<^esub>   
-      COBEGIN
-         \<lbrace>  CleanQ_RB_deq_x_P \<acute>uni \<acute>CRB bx \<rbrace>
-           \<acute>CRB := CleanQ_RB_deq_x \<acute>CRB
-         \<lbrace>  CleanQ_RB_deq_x_R \<acute>uni \<acute>CRB bx \<rbrace>, \<lbrace>True\<rbrace>
-         \<parallel> 
-         \<lbrace>  CleanQ_RB_enq_y_P \<acute>uni \<acute>CRB by \<rbrace>
-          \<acute>CRB := CleanQ_RB_enq_y by \<acute>CRB
-         \<lbrace>  CleanQ_RB_enq_y_R \<acute>uni \<acute>CRB by \<rbrace>, \<lbrace>True\<rbrace>
-      COEND
-      \<lbrace>  CleanQ_RB_Invariants \<acute>uni \<acute>CRB \<rbrace>, \<lbrace>True\<rbrace>"
-  apply(oghoare, auto)
-  apply (simp add: CleanQ_RB_enq_y_inv_all)
-  apply (simp add: CleanQ_RB_enq_y_deq_x_possible)
-  using CleanQ_RB_deq_x_all_inv apply blast
-  using CleanQ_RB_deq_x_enq_y_possible apply blast
-  apply (simp add: CleanQ_RB_enq_y_inv_all)
-  using CleanQ_RB_deq_x_all_inv apply blast
-  apply (simp add: CleanQ_RB_enq_y_inv_all)
-  apply (simp add: CleanQ_RB_enq_y_result)
-  using CleanQ_RB_deq_x_all_inv by auto
-
-lemma CleanQ_RB_deq_deq:
-     "\<Gamma>, \<Theta> |\<turnstile>\<^bsub>/F\<^esub>   
-      COBEGIN
-         \<lbrace>  CleanQ_RB_deq_x_P \<acute>uni \<acute>CRB bx \<rbrace>
-           \<acute>CRB := CleanQ_RB_deq_x \<acute>CRB
-         \<lbrace>  CleanQ_RB_deq_x_R \<acute>uni \<acute>CRB bx \<rbrace>, \<lbrace>True\<rbrace>
-         \<parallel> 
-         \<lbrace>  CleanQ_RB_deq_y_P \<acute>uni \<acute>CRB by \<rbrace>
-          \<acute>CRB := CleanQ_RB_deq_y \<acute>CRB
-         \<lbrace>  CleanQ_RB_deq_y_R \<acute>uni \<acute>CRB by \<rbrace>, \<lbrace>True\<rbrace>
-      COEND
-      \<lbrace>  CleanQ_RB_Invariants \<acute>uni \<acute>CRB \<rbrace>, \<lbrace>True\<rbrace>"
-    apply(oghoare, auto)
-  using CleanQ_RB_deq_x_all_inv apply blast
-  apply (simp add: CleanQ_RB_deq_x_no_change CleanQ_RB_deq_y_possible_def)
-  using CleanQ_RB_deq_y_all_inv apply blast
-  using CleanQ_RB_deq_y_deq_x_possible apply blast
-  using CleanQ_RB_deq_x_all_inv apply blast
-  using CleanQ_RB_deq_y_all_inv apply blast
-  using CleanQ_RB_deq_y_all_inv apply blast
-  using CleanQ_RB_deq_x_all_inv by blast
 
 lemma CleanQ_RB_loop_enq_enq:
      "\<Gamma>, \<Theta> |\<turnstile>\<^bsub>/{True}\<^esub>   
@@ -378,17 +440,16 @@ lemma CleanQ_RB_loop_enq_deq:
          \<lbrace>  CleanQ_RB_deq_y_R \<acute>uni \<acute>CRB by \<rbrace>, \<lbrace>True\<rbrace>
       COEND
       \<lbrace>  CleanQ_RB_Invariants \<acute>uni \<acute>CRB \<rbrace>, \<lbrace>True\<rbrace>"
-    apply(oghoare, auto)
-  apply (simp add: CleanQ_RB_enq_x_inv_all)
-  apply (simp add: CleanQ_RB_enq_x_deq_y_possible)
+  apply(oghoare, auto)
   apply (simp add: CleanQ_RB_deq_y_all_inv)
+  apply (simp_all add: CleanQ_RB_enq_x_deq_y_possible)
+  apply (simp_all add: CleanQ_RB_enq_x_inv_all)
   using CleanQ_RB_deq_y_enq_x_possible apply blast
-  apply (simp add: CleanQ_RB_enq_x_inv_all)
   using CleanQ_RB_deq_y_all_inv apply blast
-  apply (meson CleanQ_RB_enq_x_inv_all)
   using CleanQ_RB_deq_y_all_inv apply blast
-  apply (simp add: CleanQ_RB_enq_x_inv_all)
   using CleanQ_RB_deq_y_all_inv by blast
+  
+  
  
 lemma CleanQ_RB_loop_deq_enq:
      "\<Gamma>, \<Theta> |\<turnstile>\<^bsub>/{True}\<^esub>   
@@ -413,17 +474,15 @@ lemma CleanQ_RB_loop_deq_enq:
          \<lbrace>  CleanQ_RB_enq_y_R \<acute>uni \<acute>CRB by \<rbrace>, \<lbrace>True\<rbrace>
       COEND
       \<lbrace>  CleanQ_RB_Invariants \<acute>uni \<acute>CRB \<rbrace>, \<lbrace>True\<rbrace>" 
- apply(oghoare, auto)
-   apply (simp add: CleanQ_RB_enq_y_inv_all)
-   apply (simp add: CleanQ_RB_enq_y_deq_x_possible)
-   using CleanQ_RB_deq_x_all_inv apply blast
-   apply (simp add: CleanQ_RB_deq_x_enq_y_possible)
-   apply (simp add: CleanQ_RB_enq_y_inv_all)
-   using CleanQ_RB_deq_x_all_inv apply blast
-   apply (simp add: CleanQ_RB_enq_y_inv_all)
-   using CleanQ_RB_deq_x_all_inv apply blast
-   apply (simp add: CleanQ_RB_enq_y_inv_all)
-   using CleanQ_RB_deq_x_all_inv by blast
+  apply(oghoare, auto)
+  apply (simp_all add: CleanQ_RB_enq_y_inv_all)
+  apply (simp_all add: CleanQ_RB_enq_y_deq_x_possible)
+  using CleanQ_RB_deq_x_all_inv apply blast
+  using CleanQ_RB_deq_x_enq_y_possible apply blast
+  using CleanQ_RB_deq_x_all_inv apply blast
+  using CleanQ_RB_deq_x_all_inv apply blast
+  using CleanQ_RB_deq_x_all_inv by blast
+    
 
  lemma CleanQ_RB_loop_deq_deq:
      "\<Gamma>, \<Theta> |\<turnstile>\<^bsub>/{True}\<^esub>   
@@ -431,133 +490,32 @@ lemma CleanQ_RB_loop_deq_enq:
          \<lbrace>  CleanQ_RB_Invariants \<acute>uni \<acute>CRB \<rbrace>
          WHILE True INV \<lbrace>  CleanQ_RB_Invariants \<acute>uni \<acute>CRB \<rbrace>
          DO \<lbrace>  CleanQ_RB_Invariants \<acute>uni \<acute>CRB \<rbrace>
-           (True,\<lbrace> CleanQ_RB_deq_x_P \<acute>uni \<acute>CRB bx \<rbrace>) \<longmapsto> 
-           \<lbrace>  CleanQ_RB_deq_x_P \<acute>uni \<acute>CRB bx \<rbrace>
+           (True,\<lbrace> CleanQ_RB_deq_x_P \<acute>uni \<acute>CRB (CleanQ_RB_read_tail_x \<acute>CRB) \<rbrace>) \<longmapsto> 
+           \<lbrace>  CleanQ_RB_deq_x_P \<acute>uni \<acute>CRB (CleanQ_RB_read_tail_x \<acute>CRB)  \<rbrace>
           \<acute>CRB := CleanQ_RB_deq_x \<acute>CRB
          OD
-         \<lbrace>  CleanQ_RB_deq_x_R \<acute>uni \<acute>CRB bx \<rbrace>, \<lbrace>True\<rbrace>  
+         \<lbrace>  CleanQ_RB_deq_x_R \<acute>uni \<acute>CRB \<acute>buf_x \<rbrace>, \<lbrace>True\<rbrace>  
          \<parallel> 
          \<lbrace>  CleanQ_RB_Invariants \<acute>uni \<acute>CRB \<rbrace>
          WHILE True INV \<lbrace>  CleanQ_RB_Invariants \<acute>uni \<acute>CRB \<rbrace>
          DO
         \<lbrace>  CleanQ_RB_Invariants \<acute>uni \<acute>CRB \<rbrace>
-          (True, \<lbrace>  CleanQ_RB_deq_y_P \<acute>uni \<acute>CRB by \<rbrace>) \<longmapsto> 
-            \<lbrace>  CleanQ_RB_deq_y_P \<acute>uni \<acute>CRB by \<rbrace>
+          (True, \<lbrace>  CleanQ_RB_deq_y_P \<acute>uni \<acute>CRB (CleanQ_RB_read_tail_x \<acute>CRB) \<rbrace>) \<longmapsto> 
+            \<lbrace>  CleanQ_RB_deq_y_P \<acute>uni \<acute>CRB (CleanQ_RB_read_tail_x \<acute>CRB) \<rbrace>
             \<acute>CRB := CleanQ_RB_deq_y \<acute>CRB 
          OD
-         \<lbrace>  CleanQ_RB_deq_y_R \<acute>uni \<acute>CRB by \<rbrace>, \<lbrace>True\<rbrace>
-      COEND
-      \<lbrace>  CleanQ_RB_Invariants \<acute>uni \<acute>CRB \<rbrace>, \<lbrace>True\<rbrace>" 
- apply(oghoare, auto)
-   using CleanQ_RB_deq_x_all_inv apply blast
-   apply (simp add: CleanQ_RB_deq_x_no_change CleanQ_RB_deq_y_possible_def)
-   using CleanQ_RB_deq_y_all_inv apply blast
-   apply (simp add: CleanQ_RB_deq_y_deq_x_possible)
-   using CleanQ_RB_deq_x_all_inv apply blast
-   using CleanQ_RB_deq_y_all_inv apply blast
-   using CleanQ_RB_deq_y_all_inv apply blast
-   using CleanQ_RB_deq_x_all_inv apply blast
-   using CleanQ_RB_deq_y_all_inv apply blast
-   using CleanQ_RB_deq_x_all_inv by blast
-
- lemma CleanQ_RB_loop_all:
-     "\<Gamma>, \<Theta> |\<turnstile>\<^bsub>/{True}\<^esub>   
-      COBEGIN
-         \<lbrace>  CleanQ_RB_Invariants \<acute>uni \<acute>CRB \<rbrace>
-         WHILE True INV \<lbrace>  CleanQ_RB_Invariants \<acute>uni \<acute>CRB \<rbrace>
-         DO \<lbrace>  CleanQ_RB_Invariants \<acute>uni \<acute>CRB \<rbrace>
-           (True,\<lbrace> CleanQ_RB_deq_x_P \<acute>uni \<acute>CRB bx \<rbrace>) \<longmapsto> 
-           \<lbrace>  CleanQ_RB_deq_x_P \<acute>uni \<acute>CRB bx \<rbrace>
-           \<acute>CRB := CleanQ_RB_deq_x \<acute>CRB ;;
-           \<lbrace>  CleanQ_RB_deq_x_R \<acute>uni \<acute>CRB bx \<rbrace>
-           (True,\<lbrace> CleanQ_RB_enq_x_P \<acute>uni \<acute>CRB bx \<rbrace>) \<longmapsto> 
-           \<lbrace>  CleanQ_RB_enq_x_P \<acute>uni \<acute>CRB bx \<rbrace>
-           \<acute>CRB := CleanQ_RB_enq_x bx \<acute>CRB
-         OD
-         \<lbrace>  CleanQ_RB_enq_x_R \<acute>uni \<acute>CRB bx \<rbrace>, \<lbrace>True\<rbrace>  
-         \<parallel> 
-         \<lbrace>  CleanQ_RB_Invariants \<acute>uni \<acute>CRB \<rbrace>
-         WHILE True INV \<lbrace>  CleanQ_RB_Invariants \<acute>uni \<acute>CRB \<rbrace>
-         DO
-        \<lbrace>  CleanQ_RB_Invariants \<acute>uni \<acute>CRB \<rbrace>
-          (True, \<lbrace>  CleanQ_RB_deq_y_P \<acute>uni \<acute>CRB by \<rbrace>) \<longmapsto> 
-            \<lbrace>  CleanQ_RB_deq_y_P \<acute>uni \<acute>CRB by \<rbrace>
-            \<acute>CRB := CleanQ_RB_deq_y \<acute>CRB ;;
-           \<lbrace>  CleanQ_RB_deq_y_R \<acute>uni \<acute>CRB by \<rbrace>
-           (True,\<lbrace> CleanQ_RB_enq_y_P \<acute>uni \<acute>CRB bx \<rbrace>) \<longmapsto> 
-           \<lbrace>  CleanQ_RB_enq_y_P \<acute>uni \<acute>CRB bx \<rbrace>
-           \<acute>CRB := CleanQ_RB_enq_y bx \<acute>CRB
-         OD
-         \<lbrace>  CleanQ_RB_enq_y_R \<acute>uni \<acute>CRB by \<rbrace>, \<lbrace>True\<rbrace>
+         \<lbrace>  CleanQ_RB_deq_y_R \<acute>uni \<acute>CRB \<acute>buf_y \<rbrace>, \<lbrace>True\<rbrace>
       COEND
       \<lbrace>  CleanQ_RB_Invariants \<acute>uni \<acute>CRB \<rbrace>, \<lbrace>True\<rbrace>" 
    apply(oghoare, auto)
-   apply (meson CleanQ_RB_enq_x_inv_all)
-   apply (simp_all add: CleanQ_RB_enq_y_inv_all)
-   apply (simp_all add: CleanQ_RB_enq_x_inv_all)
-   apply (simp_all add: CleanQ_RB_deq_y_all_inv)
-   apply (simp_all add: CleanQ_RB_deq_x_all_inv)
-   apply (simp_all add: CleanQ_RB_enq_y_enq_x_possible)
-   apply (simp_all add: CleanQ_RB_enq_x_deq_y_possible)
-   apply (simp_all add: CleanQ_RB_enq_y_deq_x_possible)
-   apply (meson CleanQ_RB_enq_x_result CleanQ_RB_enq_y_buf_in_SY)
-   using CleanQ_RB_deq_x_enq_y_possible apply blast
-   using CleanQ_RB_deq_y_enq_x_possible apply blast
-   apply (simp add: CleanQ_RB_deq_x_no_change CleanQ_RB_deq_y_possible_def)
-   using CleanQ_RB_deq_y_deq_x_possible by blast
+   apply (simp_all add: CleanQ_RB_deq_x_no_change CleanQ_RB_deq_y_possible_def)
+   apply (simp_all add: CleanQ_RB_deq_y_deq_x_possible)
+   using CleanQ_RB_deq_x_all_inv apply blast
+   apply (simp_all add: CleanQ_RB_deq_y_all_inv CleanQ_RB_deq_y_possible_def)
+   using CleanQ_RB_deq_x_all_inv apply blast
+   using CleanQ_RB_deq_x_all_inv apply blast
+   using CleanQ_RB_deq_x_all_inv by blast
   
-   
-(* Different order of operations *) 
-
-lemma CleanQ_RB_loop_all2:
-     "\<Gamma>, \<Theta> |\<turnstile>\<^bsub>/{True}\<^esub>   
-      COBEGIN
-         \<lbrace>  CleanQ_RB_Invariants \<acute>uni \<acute>CRB \<rbrace>
-         WHILE True INV \<lbrace>  CleanQ_RB_Invariants \<acute>uni \<acute>CRB \<rbrace>
-         DO \<lbrace>  CleanQ_RB_Invariants \<acute>uni \<acute>CRB \<rbrace>
-           (True,\<lbrace> CleanQ_RB_enq_x_P \<acute>uni \<acute>CRB bx \<rbrace>) \<longmapsto> 
-           \<lbrace>  CleanQ_RB_enq_x_P \<acute>uni \<acute>CRB bx \<rbrace>
-           \<acute>CRB := CleanQ_RB_enq_x bx \<acute>CRB;;
-           \<lbrace>  CleanQ_RB_enq_x_R \<acute>uni \<acute>CRB bx \<rbrace>
-           (True,\<lbrace> CleanQ_RB_deq_x_P \<acute>uni \<acute>CRB bx \<rbrace>) \<longmapsto> 
-           \<lbrace>  CleanQ_RB_deq_x_P \<acute>uni \<acute>CRB bx \<rbrace>
-           \<acute>CRB := CleanQ_RB_deq_x \<acute>CRB
-         OD
-         \<lbrace>  CleanQ_RB_deq_x_R \<acute>uni \<acute>CRB bx \<rbrace>, \<lbrace>True\<rbrace>  
-         \<parallel> 
-         \<lbrace>  CleanQ_RB_Invariants \<acute>uni \<acute>CRB \<rbrace>
-         WHILE True INV \<lbrace>  CleanQ_RB_Invariants \<acute>uni \<acute>CRB \<rbrace>
-         DO
-        \<lbrace>  CleanQ_RB_Invariants \<acute>uni \<acute>CRB \<rbrace>
-          (True, \<lbrace>  CleanQ_RB_enq_y_P \<acute>uni \<acute>CRB by \<rbrace>) \<longmapsto> 
-            \<lbrace>  CleanQ_RB_enq_y_P \<acute>uni \<acute>CRB by \<rbrace>
-            \<acute>CRB := CleanQ_RB_enq_y by \<acute>CRB ;;
-           \<lbrace>  CleanQ_RB_enq_y_R \<acute>uni \<acute>CRB by \<rbrace>
-           (True,\<lbrace> CleanQ_RB_deq_y_P \<acute>uni \<acute>CRB bx \<rbrace>) \<longmapsto> 
-           \<lbrace>  CleanQ_RB_deq_y_P \<acute>uni \<acute>CRB bx \<rbrace>
-           \<acute>CRB := CleanQ_RB_deq_y \<acute>CRB
-         OD
-         \<lbrace>  CleanQ_RB_deq_y_R \<acute>uni \<acute>CRB by \<rbrace>, \<lbrace>True\<rbrace>
-      COEND
-      \<lbrace>  CleanQ_RB_Invariants \<acute>uni \<acute>CRB \<rbrace>, \<lbrace>True\<rbrace>" 
-  apply(oghoare, auto)
-  apply (meson CleanQ_RB_enq_x_inv_all)
-  apply (simp_all add: CleanQ_RB_enq_x_inv_all)
-  apply (simp_all add: CleanQ_RB_enq_y_inv_all)
-  apply(simp_all add: CleanQ_RB_deq_x_all_inv)
-  apply(simp_all add: CleanQ_RB_deq_y_all_inv)
-  apply(simp_all add: CleanQ_RB_enq_y_result)
-  apply(simp_all add: CleanQ_RB_enq_x_result)
-  apply(simp_all add: CleanQ_RB_deq_x_enq_y_possible)
-  apply (simp add: CleanQ_RB_enq_x_def CleanQ_RB_enq_y_possible_def)
-  apply (simp add: CleanQ_RB_enq_y_enq_x_possible CleanQ_RB_enq_y_possible_def)
-  apply (simp add: CleanQ_RB_enq_x_deq_y_possible)
-  apply (simp add: CleanQ_RB_enq_y_deq_x_possible)
-  using CleanQ_RB_deq_y_enq_x_possible apply blast
-  apply (simp add: CleanQ_RB_deq_x_no_change CleanQ_RB_deq_y_possible_def)
-  by (simp add: CleanQ_RB_deq_y_deq_x_possible)
-
-
 lemma CleanQ_RB_concurrent_all:
      "\<Gamma>, \<Theta> |\<turnstile>\<^bsub>/{True}\<^esub>   
       COBEGIN
@@ -570,13 +528,13 @@ lemma CleanQ_RB_concurrent_all:
             \<lbrace> CleanQ_RB_enq_x_Q \<acute>uni \<acute>CRB bx \<rbrace>
               \<acute>CRB := (CleanQ_RB_incr_head_x bx \<acute>CRB)) ;;
             \<lbrace>  CleanQ_RB_Invariants \<acute>uni \<acute>CRB \<rbrace>
-              (True,\<lbrace> CleanQ_RB_deq_x_P \<acute>uni \<acute>CRB bx2 \<rbrace>) \<longmapsto> ( 
-            \<lbrace> CleanQ_RB_deq_x_P \<acute>uni \<acute>CRB bx2 \<rbrace>
-              \<acute>buf := (CleanQ_RB_read_tail_x \<acute>CRB) ;;
-            \<lbrace> CleanQ_RB_deq_x_Q \<acute>uni \<acute>CRB bx2 \<rbrace>
-             \<acute>CRB := (CleanQ_RB_incr_tail_x bx2 \<acute>CRB))
+              (True,\<lbrace> CleanQ_RB_deq_x_P \<acute>uni \<acute>CRB (CleanQ_RB_read_tail_x \<acute>CRB) \<rbrace>) \<longmapsto> ( 
+            \<lbrace> CleanQ_RB_deq_x_P \<acute>uni \<acute>CRB (CleanQ_RB_read_tail_x \<acute>CRB) \<rbrace>
+              \<acute>buf_x := (CleanQ_RB_read_tail_x \<acute>CRB) ;;
+            \<lbrace> CleanQ_RB_deq_x_Q \<acute>uni \<acute>CRB \<acute>buf_x \<rbrace>
+             \<acute>CRB := (CleanQ_RB_incr_tail_x \<acute>buf_x \<acute>CRB))
          OD
-         \<lbrace>  CleanQ_RB_deq_x_R \<acute>uni \<acute>CRB bx2 \<rbrace>, \<lbrace>True\<rbrace>  
+         \<lbrace>  CleanQ_RB_deq_x_R \<acute>uni \<acute>CRB \<acute>buf_x \<rbrace>, \<lbrace>True\<rbrace>  
          \<parallel> 
          \<lbrace>  CleanQ_RB_Invariants \<acute>uni \<acute>CRB \<rbrace>
          WHILE True INV \<lbrace>  CleanQ_RB_Invariants \<acute>uni \<acute>CRB \<rbrace>
@@ -587,34 +545,58 @@ lemma CleanQ_RB_concurrent_all:
             \<lbrace> CleanQ_RB_enq_y_Q \<acute>uni \<acute>CRB by \<rbrace>
               \<acute>CRB := (CleanQ_RB_incr_head_y by \<acute>CRB)) ;;
             \<lbrace>  CleanQ_RB_Invariants \<acute>uni \<acute>CRB \<rbrace>
-              (True,\<lbrace> CleanQ_RB_deq_y_P \<acute>uni \<acute>CRB by2 \<rbrace>) \<longmapsto> ( 
-            \<lbrace> CleanQ_RB_deq_y_P \<acute>uni \<acute>CRB by2 \<rbrace>
-              \<acute>buf := (CleanQ_RB_read_tail_y \<acute>CRB) ;;
-            \<lbrace> CleanQ_RB_deq_y_Q \<acute>uni \<acute>CRB by2 \<rbrace>
-             \<acute>CRB := (CleanQ_RB_incr_tail_y by2 \<acute>CRB))
+              (True,\<lbrace> CleanQ_RB_deq_y_P \<acute>uni \<acute>CRB (CleanQ_RB_read_tail_y \<acute>CRB) \<rbrace>) \<longmapsto> ( 
+            \<lbrace> CleanQ_RB_deq_y_P \<acute>uni \<acute>CRB (CleanQ_RB_read_tail_y \<acute>CRB) \<rbrace>
+              \<acute>buf_y := (CleanQ_RB_read_tail_y \<acute>CRB) ;;
+            \<lbrace> CleanQ_RB_deq_y_Q \<acute>uni \<acute>CRB \<acute>buf_y \<rbrace>
+             \<acute>CRB := (CleanQ_RB_incr_tail_y \<acute>buf_y \<acute>CRB))
          OD
-         \<lbrace>  CleanQ_RB_deq_y_R \<acute>uni \<acute>CRB by2 \<rbrace>, \<lbrace>True\<rbrace>
+         \<lbrace>  CleanQ_RB_deq_y_R \<acute>uni \<acute>CRB \<acute>buf_y \<rbrace>, \<lbrace>True\<rbrace>
       COEND
       \<lbrace>  CleanQ_RB_Invariants \<acute>uni \<acute>CRB \<rbrace>, \<lbrace>True\<rbrace>" 
   apply(oghoare, auto)
   apply (simp_all add: CleanQ_RB_enq_x_inv_all)
   apply (simp_all add: CleanQ_RB_enq_y_inv_all)
-  apply (simp_all add: CleanQ_RB_deq_x_all_inv CleanQ_RB_deq_x_equiv_incr_tail)
-  apply (simp_all add: CleanQ_RB_deq_x_no_change CleanQ_RB_deq_y_possible_def)
-  apply (simp_all add: CleanQ_RB_deq_y_all_inv CleanQ_RB_deq_y_equiv_incr_tail CleanQ_RB_deq_y_possible_def)
-  apply (simp_all add: CleanQ_RB_deq_y_deq_x_possible)
-  apply (simp_all add: CleanQ_RB_enq_x_def)
-  apply (simp_all add: CleanQ_RB_enq_y_def)
   apply (simp_all add: CleanQ_RB_enq_x_def CleanQ_RB_enq_y_possible_def)
-  apply (simp_all add: CleanQ_RB_enq_x_possible_def)
-  apply (simp_all add: CleanQ_RB_Invariants_def I4_rb_valid_def)
-  apply (simp_all add: CleanQ_RB_deq_x_possible_def)
-  apply (meson CleanQ_RB_Invariants_def CleanQ_RB_deq_x_enq_y_possible CleanQ_RB_deq_x_possible_def CleanQ_RB_enq_y_possible_def I4_rb_valid_def)
-  using CleanQ_RB_Invariants_def CleanQ_RB_deq_y_enq_x_possible CleanQ_RB_deq_y_possible_def CleanQ_RB_enq_x_possible_def I4_rb_valid_def apply blast
-  using CleanQ_RB_Invariants_def CleanQ_RB_deq_x_enq_y_possible CleanQ_RB_deq_x_possible_def CleanQ_RB_enq_y_possible_def I4_rb_valid_def apply blast
-  using CleanQ_RB_Invariants_def CleanQ_RB_deq_y_enq_x_possible CleanQ_RB_deq_y_possible_def CleanQ_RB_enq_x_possible_def I4_rb_valid_def apply blast
-  using CleanQ_RB_Invariants_def CleanQ_RB_deq_x_enq_y_possible CleanQ_RB_deq_x_possible_def CleanQ_RB_enq_y_possible_def I4_rb_valid_def apply blast
-  using CleanQ_RB_Invariants_def CleanQ_RB_deq_y_enq_x_possible CleanQ_RB_deq_y_possible_def CleanQ_RB_enq_x_possible_def I4_rb_valid_def by blast
+  apply (simp_all add: CleanQ_RB_enq_y_enq_x_possible CleanQ_RB_enq_y_possible_def)
+  using CleanQ_RB_deq_x_all_inv apply blast
+  using CleanQ_RB_deq_y_all_inv apply blast
+  using CleanQ_RB_deq_x_all_inv apply blast
+  using CleanQ_RB_deq_x_enq_y_possible CleanQ_RB_enq_y_possible_def apply blast
+  using CleanQ_RB_deq_y_all_inv apply blast
+  using CleanQ_RB_deq_y_enq_x_possible apply blast
+  apply (metis CleanQ_RB_enq_x_def CleanQ_RB_enq_x_deq_y_possible)
+  apply (simp add: CleanQ_RB_enq_y_deq_x_possible CleanQ_RB_enq_y_possible_def)
+  using CleanQ_RB_deq_x_all_inv apply blast
+  apply (simp add: CleanQ_RB_deq_x_no_change CleanQ_RB_deq_y_possible_def)
+  using CleanQ_RB_deq_y_all_inv apply blast
+  using CleanQ_RB_deq_y_deq_x_possible apply blast
+  using CleanQ_RB_deq_x_all_inv apply blast
+  using CleanQ_RB_deq_x_enq_y_possible CleanQ_RB_enq_y_possible_def apply blast
+  using CleanQ_RB_deq_y_all_inv apply blast
+  using CleanQ_RB_deq_y_enq_x_possible apply blast
+  apply (simp add: CleanQ_RB_Invariants_def CleanQ_RB_deq_y_possible_def CleanQ_RB_enq_x_possible_def I4_rb_valid_def)
+  apply (simp add: CleanQ_RB_enq_y_deq_x_possible CleanQ_RB_enq_y_possible_def)
+  using CleanQ_RB_deq_x_all_inv apply blast
+  apply (simp add: CleanQ_RB_deq_x_no_change CleanQ_RB_deq_y_possible_def)
+  using CleanQ_RB_deq_y_all_inv apply blast
+  using CleanQ_RB_deq_y_deq_x_possible apply blast
+  using CleanQ_RB_deq_x_all_inv apply blast
+  using CleanQ_RB_deq_x_enq_y_possible CleanQ_RB_enq_y_possible_def apply blast
+  using CleanQ_RB_deq_y_all_inv apply blast
+  using CleanQ_RB_deq_y_enq_x_possible apply blast
+  using CleanQ_RB_deq_x_all_inv apply blast
+  using CleanQ_RB_deq_y_all_inv apply blast
+  apply (metis CleanQ_RB_enq_x_def CleanQ_RB_enq_x_deq_y_possible)
+  apply (simp add: CleanQ_RB_enq_y_deq_x_possible CleanQ_RB_enq_y_possible_def)
+  using CleanQ_RB_deq_x_all_inv apply blast
+  apply (simp add: CleanQ_RB_deq_x_no_change CleanQ_RB_deq_y_possible_def)
+  using CleanQ_RB_deq_y_all_inv apply blast
+  using CleanQ_RB_deq_y_deq_x_possible apply blast
+  using CleanQ_RB_deq_y_all_inv apply blast
+  using CleanQ_RB_deq_x_all_inv apply blast
+  using CleanQ_RB_deq_y_all_inv apply blast
+  using CleanQ_RB_deq_x_all_inv by blast
 
 
 lemma CleanQ_RB_concurrent_if_all:
@@ -622,55 +604,17 @@ lemma CleanQ_RB_concurrent_if_all:
       COBEGIN
          \<lbrace>  CleanQ_RB_Invariants \<acute>uni \<acute>CRB \<rbrace>
          WHILE True INV \<lbrace>  CleanQ_RB_Invariants \<acute>uni \<acute>CRB \<rbrace>
-         DO \<lbrace>  CleanQ_RB_Invariants \<acute>uni \<acute>CRB \<rbrace>
-            IF CleanQ_RB_enq_x_possible \<acute>CRB \<and> bx \<in> rSX \<acute>CRB
-            THEN
-              \<lbrace> CleanQ_RB_enq_x_P \<acute>uni \<acute>CRB bx \<rbrace>
-                \<acute>CRB := (CleanQ_RB_write_head_x bx \<acute>CRB) ;;
-              \<lbrace> CleanQ_RB_enq_x_Q \<acute>uni \<acute>CRB bx \<rbrace>
-                \<acute>CRB := (CleanQ_RB_incr_head_x bx \<acute>CRB)
-            ELSE 
-                \<lbrace>  CleanQ_RB_Invariants \<acute>uni \<acute>CRB \<rbrace>
-                SKIP
-            FI;;
-            \<lbrace>  CleanQ_RB_Invariants \<acute>uni \<acute>CRB \<rbrace>
-            IF CleanQ_RB_deq_x_possible \<acute>CRB \<and> bx2 = CleanQ_RB_read_tail_x \<acute>CRB
-            THEN
-              \<lbrace> CleanQ_RB_deq_x_P \<acute>uni \<acute>CRB bx2 \<rbrace>
-                \<acute>buf := (CleanQ_RB_read_tail_x \<acute>CRB) ;;
-              \<lbrace> CleanQ_RB_deq_x_Q \<acute>uni \<acute>CRB bx2 \<rbrace>
-               \<acute>CRB := (CleanQ_RB_incr_tail_x bx2 \<acute>CRB)
-            ELSE 
-                \<lbrace>  CleanQ_RB_Invariants \<acute>uni \<acute>CRB \<rbrace>
-                SKIP
-            FI
+         DO  
+            CleanQ_CRB_enq_x b;;
+            CleanQ_CRB_deq_x
          OD
          \<lbrace>  CleanQ_RB_Invariants \<acute>uni \<acute>CRB \<rbrace>, \<lbrace>True\<rbrace>  
          \<parallel> 
          \<lbrace>  CleanQ_RB_Invariants \<acute>uni \<acute>CRB \<rbrace>
          WHILE True INV \<lbrace>  CleanQ_RB_Invariants \<acute>uni \<acute>CRB \<rbrace>
-         DO \<lbrace>  CleanQ_RB_Invariants \<acute>uni \<acute>CRB \<rbrace>
-            IF CleanQ_RB_enq_y_possible \<acute>CRB \<and> by \<in> rSY \<acute>CRB
-            THEN
-              \<lbrace> CleanQ_RB_enq_y_P \<acute>uni \<acute>CRB by \<rbrace>
-                \<acute>CRB := (CleanQ_RB_write_head_y by \<acute>CRB) ;;
-              \<lbrace> CleanQ_RB_enq_y_Q \<acute>uni \<acute>CRB by \<rbrace>
-                \<acute>CRB := (CleanQ_RB_incr_head_y by \<acute>CRB)
-            ELSE 
-                \<lbrace>  CleanQ_RB_Invariants \<acute>uni \<acute>CRB \<rbrace>
-                SKIP
-            FI;;
-            \<lbrace>  CleanQ_RB_Invariants \<acute>uni \<acute>CRB \<rbrace>
-            IF CleanQ_RB_deq_y_possible \<acute>CRB \<and> by2 = CleanQ_RB_read_tail_y \<acute>CRB
-            THEN
-              \<lbrace> CleanQ_RB_deq_y_P \<acute>uni \<acute>CRB by2 \<rbrace>
-                \<acute>buf := (CleanQ_RB_read_tail_y \<acute>CRB) ;;
-              \<lbrace> CleanQ_RB_deq_y_Q \<acute>uni \<acute>CRB by2 \<rbrace>
-               \<acute>CRB := (CleanQ_RB_incr_tail_y by2 \<acute>CRB)
-            ELSE 
-                \<lbrace>  CleanQ_RB_Invariants \<acute>uni \<acute>CRB \<rbrace>
-                SKIP
-            FI
+         DO 
+            CleanQ_CRB_enq_y b2;;
+            CleanQ_CRB_deq_y
          OD
          \<lbrace>  CleanQ_RB_Invariants \<acute>uni \<acute>CRB \<rbrace>, \<lbrace>True\<rbrace>
       COEND
@@ -678,20 +622,27 @@ lemma CleanQ_RB_concurrent_if_all:
   apply(oghoare, auto)
   apply (simp_all add: CleanQ_RB_enq_x_inv_all)
   apply (simp_all add: CleanQ_RB_enq_y_inv_all)
+  apply (simp_all add: CleanQ_RB_enq_y_enq_x_possible)
+  apply (simp_all add: CleanQ_RB_enq_x_deq_y_possible)
+  using CleanQ_RB_deq_x_all_inv apply blast
+  using CleanQ_RB_deq_y_all_inv apply blast
+  apply (simp_all add: CleanQ_RB_enq_y_deq_x_possible)
   apply (simp_all add: CleanQ_RB_deq_x_all_inv CleanQ_RB_deq_x_equiv_incr_tail)
   apply (simp_all add: CleanQ_RB_deq_x_no_change CleanQ_RB_deq_y_possible_def)
   apply (simp_all add: CleanQ_RB_deq_y_all_inv CleanQ_RB_deq_y_equiv_incr_tail CleanQ_RB_deq_y_possible_def)
-  apply (simp_all add: CleanQ_RB_deq_y_deq_x_possible)
-  apply (simp_all add: CleanQ_RB_enq_x_def)
-  apply (simp_all add: CleanQ_RB_enq_y_def)
   apply (simp_all add: CleanQ_RB_enq_x_def CleanQ_RB_enq_y_possible_def)
-  apply (simp_all add: CleanQ_RB_enq_x_possible_def)
-  apply (simp_all add: CleanQ_RB_Invariants_def I4_rb_valid_def)
-  apply (simp_all add: CleanQ_RB_deq_x_possible_def)
-  apply (simp_all add: CleanQ_RB_deq_x_def case_prod_unfold)
-  using CleanQ_RB_Invariants_def CleanQ_RB_deq_y_enq_x_possible 
-    CleanQ_RB_deq_y_possible_def CleanQ_RB_enq_x_possible_def I4_rb_valid_def apply blast
-  by (simp_all add: CleanQ_RB_deq_y_def case_prod_unfold)
+  using CleanQ_RB_deq_x_enq_y_possible CleanQ_RB_enq_y_possible_def apply blast
+  apply (simp_all add: CleanQ_RB_deq_y_enq_x_possible CleanQ_RB_deq_y_possible_def)
+  using CleanQ_RB_deq_y_deq_x_possible apply blast
+  using CleanQ_RB_deq_x_enq_y_possible CleanQ_RB_enq_y_possible_def apply blast
+  using CleanQ_RB_deq_y_deq_x_possible apply blast
+  using CleanQ_RB_deq_x_enq_y_possible CleanQ_RB_enq_y_possible_def apply blast
+  using CleanQ_RB_deq_y_deq_x_possible by blast
+
+
+  
+  
+  
   
   
 
